Cleanup

theories/examples/DemoLogSemSeminar.v
@@ -1,10 +1,8 @@
-Require Import String Basics.
+Require Import String Basics ZArith.
 Require Import List.
-Require Import Ast Notations EvalE PCUICtoTemplate PCUICTranslate.
+Require Import Ast Notations EvalE PCUICtoTemplate PCUICTranslate AcornExamples.
 
 From MetaCoq.Template Require Ast.
-(* From MetaCoq.Template Require Import TemplateMonad. *)
-(* From MetaCoq.Template Require Import monad_utils. *)
 
 Definition expr_to_tc Σ := compose trans (expr_to_term Σ).
 Definition type_to_tc := compose trans type_to_term.
@@ -13,7 +11,6 @@ Definition global_to_tc := compose trans_minductive_entry trans_global_dec.
 Import ListNotations.
 Module TC := Template.BasicAst.
 
-(* Import MonadNotation. *)
 Import BaseTypes.
 Import StdLib.
 
@@ -57,20 +54,107 @@ Set Printing Notations.
 (* Execute the program using the interpreter *)
 Compute (expr_eval_n Σ 3 nil [|{my_negb_syn} True |]).
 
-Compute (expr_eval_i Σ 3 nil (indexify nil negb_app_true)).
+Compute (expr_eval_i Σ 3 nil (indexify nil [|{my_negb_syn} True |])).
 
 
 (* Make a Coq function from the AST of the program *)
-Make Definition coq_negb_app_true :=
-  (expr_to_tc Σ (indexify nil negb_app_true)).
-
-Print coq_negb_app_true.
-
 Make Definition my_negb :=
   (expr_to_tc Σ (indexify nil my_negb_syn)).
 
+Print my_negb.
+
+(** [my_neg] is equivalent to [negb] from the standard library *)
 Lemma my_negb_coq_negb b :
   my_negb b = negb b.
 Proof. reflexivity. Qed.
 
-Compute (expr_eval_n Σ 3 nil my_negb_syn).
+Module CounterContract.
+  (** Concrete syntax in Acorn *)
+
+  (*
+  module CoqExamples where
+
+  import Prim
+
+  data Msg = Inc [Int64] | Dec [Int64]
+
+  data CState = CState [Int64, {address}]
+
+  definition owner (s :: CState) =
+     case s of
+       CState _ d -> d
+
+  definition balance (s :: CState) =
+     case s of
+       CState x _ -> x
+
+  definition count (s :: CState) (msg :: Msg) =
+    case msg of
+      Inc a ->
+        CState (Prim.plusInt64 (balance s) a) (owner s)
+      Dec a ->
+        CState (Prim.minusInt64 (balance s) a) (owner s)
+   *)
+
+  (** AST of Data type definitions and functions corresponding to the module [CoqExamples] above *)
+  Definition CounterData := [gdInd "Msg" 0 [("Inc_coq", [(None, tyInd "Z")]);("Dec_coq", [(None, tyInd "Z")])] false;gdInd "CState" 0 [("CState_coq", [(None, tyInd "Z");(None, tyInd "string")])] false].
+  (*---------------------*)
+  Definition CounterFunctions := [("owner", eLambda "x" ((tyInd "CState")) (eCase ("CState", []) (tyInd "string") (eRel 0) [(pConstr "CState_coq" ["x0";"x1"], eRel 0)])) ;("balance", eLambda "x" ((tyInd "CState")) (eCase ("CState", []) (tyInd "Z") (eRel 0) [(pConstr "CState_coq" ["x0";"x1"], eRel 1)])); ("count", eLambda "x" ((tyInd "ReceiveContext")) (eLambda "x" ((tyInd "CState")) (eLambda "x" ((tyInd "Caller")) (eLambda "x" (tyInd "nat") (eLambda "x" ((tyApp (tyInd "Maybe") ((tyInd "Msg")))) (eCase ("Maybe", [(tyInd "Msg")]) ((tyApp (tyApp (tyInd "Pair") ((tyInd "CState"))) ((tyInd "Transaction")))) (eRel 0) [(pConstr "Nothing_coq" [], eApp (eApp (eApp (eApp (eConstr "Pair" "Pair_coq") (eTy ((tyInd "CState")))) (eTy ((tyInd "Transaction")))) (eRel 3)) (eConst "TxNone")); (pConstr "Just_coq" ["x0"], eCase ("Msg", []) ((tyApp (tyApp (tyInd "Pair") ((tyInd "CState"))) ((tyInd "Transaction")))) (eRel 0) [(pConstr "Inc_coq" ["x0"], eLetIn "x" (eApp (eApp (eConstr "CState" "CState_coq") (eApp (eApp (eConst "plusInt64") (eApp (eConst "balance") (eRel 5))) (eRel 0))) (eApp (eConst "owner") (eRel 5))) ((tyInd "CState")) (eApp (eApp (eApp (eApp (eConstr "Pair" "Pair_coq") (eTy ((tyInd "CState")))) (eTy ((tyInd "Transaction")))) (eRel 0)) (eConst "TxNone"))); (pConstr "Dec_coq" ["x0"], eLetIn "x" (eApp (eApp (eConstr "CState" "CState_coq") (eApp (eApp (eConst "minusInt64") (eApp (eConst "balance") (eRel 5))) (eRel 0))) (eApp (eConst "owner") (eRel 5))) ((tyInd "CState")) (eApp (eApp (eApp (eApp (eConstr "Pair" "Pair_coq") (eTy ((tyInd "CState")))) (eTy ((tyInd "Transaction")))) (eRel 0)) (eConst "TxNone")))])]))))))].
+
+  (** We assume that primitive data types are available *)
+  Module Prim.
+    Inductive Transaction := txNone.
+    Definition plusInt64 := Z.add.
+    Definition minusInt64 := Z.sub.
+    Definition TxNone := txNone.
+  End Prim.
+
+  (** We import Acorn "standard library" definitions before unquoting. These definitions were also produced by the same printing procedure.  *)
+  Import Prim.
+  Import AcornProd.
+  Import AcornMaybe.
+  Import AcornBlockchain.
+
+  (** Now, we add all data types, required for the translation of the [counter] to the global environment *)
+  Definition gEnv := ((StdLib.Σ ++ AcornMaybe.Data ++ AcornBlockchain.Data ++ AcornProd.Data ++ CounterData)%list).
+
+  (** We translate data types and the [counter] contract to MetaCoq and unquote them using the template moand *)
+  Run TemplateProgram (translateData CounterData).
+  Run TemplateProgram (translateDefs gEnv CounterFunctions).
+
+  (** After that, we can interact with the shallow embedding in a usual way *)
+  Print Msg.
+  (* Inductive Msg : Set :=  Inc_coq : Z -> Msg | Dec_coq : Z -> Msg *)
+
+  Print count.
+(* count =
+  fun _ x0 _ _ x3 =>
+  match x3 with
+   | @Nothing_coq _ => Pair_coq CState Transaction x0 TxNone
+   | @Just_coq _ (Inc_coq x5) =>
+      Pair_coq CState Transaction
+       (CState_coq (plusInt64 (balance x0) x5) (owner x0)) TxNone
+   | @Just_coq _ (Dec_coq x5) =>
+      Pair_coq CState Transaction
+       (CState_coq (minusInt64 (balance x0) x5) (owner x0)) TxNone
+  end
+     : ReceiveContext -> CState -> Caller
+       -> nat -> Maybe Msg -> Pair CState Transaction *)
+
+  Open Scope Z_scope.
+
+  (** Using the shallow embedding, we can show a simple functional correctness property *)
+  Lemma inc_correct init n i fin tx ctx amount caller :
+    (* precondition *)
+    balance init = n ->
+
+    (* sending "increment" *)
+    count ctx init caller amount (Just_coq _ (Inc_coq i)) = Pair_coq _ _ fin tx ->
+
+    (* result *)
+    balance fin = n + i.
+  Proof.
+    intros Hinit Hrun. inversion Hrun. subst. reflexivity.
+  Qed.
+
+End CounterContract.
